\documentclass{ximera}

\input{../../preamble.tex}

\title{Solving Equations}

\begin{document}

\begin{abstract}
break it up
\end{abstract}
\maketitle





\begin{example}  Common Factor


Solve $\sqrt{x+9} + x \cdot \frac{1}{2} (x+9)^{-\tfrac{1}{2}} = 0$



\begin{explanation}



A common factor is a factor of the least degree in all of the terms.  We have one here. $(x+9)$ is a factor in both terms.  The powers are $\frac{1}{2}$ and $-\frac{1}{2}$. The least of which is $-\frac{1}{2}$.

We will use the distributive property to factor out $(x+9)^{\answer{-\frac{1}{2}}}$.


$(x+9)^{-\tfrac{1}{2}} \left((x+9) + x \cdot \frac{1}{2}\right)  = 0$


We could, in turn, write this as a fraction


\[  \frac{\left((x+9) + x \cdot \frac{1}{2}\right)}{\sqrt{x+9}} = 0 \]


\[  \frac{ \frac{3}{2} x + 9}{\sqrt{x+9}} = 0 \]



This is a fraction, so it equals $0$ when the numerator equals $0$ and the denominator does not equal $0$.


$\answer{\frac{3}{2} x + 9} = 0$



$x = -6$, which is in the domain of $\sqrt{x+9} + x \cdot \frac{1}{2} (x+9)^{-\tfrac{1}{2}}$.


\end{explanation}
\end{example}




Incidentally, $\sqrt{x+9} + x \cdot \frac{1}{2} (x+9)^{-\tfrac{1}{2}}$ is the derivative of $\sqrt{x+9}$.  So, we are finding where $\sqrt{x+9}$ switches between increasing and decreasing.






\begin{example}  Common Denominator

\begin{explanation}


Factoring out a common factor can also be viewed as getting a common denominator and combining into a single fraction. \\


\[
\sqrt{x+9} + x \cdot \frac{1}{2} (x+9)^{-\tfrac{1}{2}} = \sqrt{x+9} + x \cdot \frac{1}{2 \, \sqrt{x+9}} = \frac{2(x+9)}{2 \, \sqrt{x+9}} +  \frac{x}{2 \, \sqrt{x+9}}   
\]


\[
= \frac{2 \, (x + 9) + x}{2 \, \sqrt{x+9}}   
\]


\[
= \frac{3x + 18}{2 \, \sqrt{x+9}}   
\]


\[
= \frac{3 \, (x + 6)}{2 \, \sqrt{x+9}}   
\]

\end{explanation}
\end{example}









\begin{example}  Common Factor


Solve 

\[  \frac{x^3 (18x) - 9(x^2-3)(3x^2)}{(x^3)^2} = 0 \]



\begin{explanation}


The numerator is a difference of two terms and $9 x^2$ is a common factor.  We can use the Distributive Property to factor it out.



\[  \frac{9x^2 (2x^2 - 3(x^2-3))}{x^6} = 0  \]


\[  \frac{9 \left( \answer{9 - x^2} \right)}{x^4} = 0 \]



This is a fraction, so it equals $0$ when the numerator equals $0$ and the denominator does not equal $0$.


$9 - x^2 = 0$

This has two solutions: $\{ -3, 3  \}$, both of which are in the domain.






\end{explanation}

\end{example}





Incidentally, $\frac{x^3 (18x) - 9(x^2-3)(3x^2)}{(x^3)^2}$ is the derivative of $\frac{9(x^2-3)}{x^3}$.  So, we are finding where $\frac{9(x^2-3)}{x^3}$ switches between increasing and decreasing.











\begin{example}  Common Factor


Solve $12 x^3 - 12 x^2 = 0 $



\begin{explanation}


The Distributive Property (factoring) gives us the product $12 x^2 (x-1)$.




We have two solutions: $\{ 0, 1  \}$, both of which are in the domain.


\end{explanation}


$12 x^3 - 12 x^2$ is the derivative of $3x^4 - 4x^3$.  Therefore, the graph of $y = 3x^4 - 4x^3$ has horizontal tangent lines at $(0, 0)$ and $(1, -1)$.





\begin{center}
\desmos{ugpotyh1qa}{400}{300}
\end{center}


\end{example}





















\begin{example}  Fractions


Solve $2 - \frac{2}{\sqrt[3]{x}} = 0$



\begin{explanation}


Converting to exponents gives us $2 - \frac{2}{x^{\tfrac{1}{3}}} = 0$


$2 = \frac{2}{x^{\tfrac{1}{3}}}$

The only way this can happen is if $x^{\tfrac{1}{3}} = \answer{1}$.

This has one solution: $\{  1  \}$





\end{explanation}


\end{example}











\begin{center}
\textbf{\textcolor{green!50!black}{ooooo-=-=-=-ooOoo-=-=-=-ooooo}} \\

more examples can be found by following this link\\ \link[More Examples of Function Zeros]{https://ximera.osu.edu/csccmathematics/precalculus1/precalculus1/zeros/examples/exampleList}

\end{center}






\end{document}
