\documentclass{ximera}

\input{../../preamble.tex}

\title{Closed Form}

\begin{document}

\begin{abstract}
center
\end{abstract}
\maketitle






Let's walk the bridge backwards



\section*{Closed Form}



\begin{example} Gemetric Series


Given 
\[    K(t) =   \sum_{n=0}^{\infty}  \left( \frac{t}{2} \right)^2\]

find the closed form formula and the interval of convergence.




\begin{explanation}


This is a Geometric series.  The interval of convergence is $(-2, 2)$, since this is when the inside of the general term is $-1$ and $1$.


The closed form is

\[  \frac{1}{1 - \frac{t}{2}}  =     \frac{2}{2-t}           \]



\end{explanation}


\end{example}




The infinite geometric series will equal $\frac{2}{2-t}$ on $(-2, 2)$.  How many terms of the series to we need for a good approximation on just $(-0.75, 0.75)$?



\begin{center}
\desmos{oy88ukjmwc}{400}{300}
\end{center}






\begin{example} Gemetric Series


Given 
\[    K(t) =   \sum_{n=2}^{\infty}  \left( \frac{t}{2} \right)^2    \]

find the closed form formula and the interval of convergence.




\begin{explanation}


This is the same Geometric series, except missing the first two terms.  The interval of convergence is $(-2, 2)$, since this is when the inside of the general term is $-1$ and $1$.


The closed form is the same, except subtract off the first two terms.

\[  \frac{1}{1 - \frac{t}{2}}  - 1 - \frac{t}{2}    =     \frac{2}{2-t}  - 1 - \frac{t}{2}     \]


need a common denominator


\[=     \frac{4}{2(2-t)}  - \frac{2(2-t)}{2(2-t)} - \frac{t(2-t)}{2(2-t)} = \frac{4-2(2-t)-t(2-t)}{2(2-t)}  = \frac{t^2}{2(2-t)}   \]





\[    K(t) =   \frac{t^2}{2(2-t)}    \] on $(-2, 2)$.


\end{explanation}

\end{example}




On the other hand, we could have factored out $\left( \frac{t}{2} \right)$ in order to get the index back to $0$.


\[    K(t) =   \sum_{n=2}^{\infty}  \left( \frac{t}{2} \right)^n    =  \left( \frac{t}{2} \right)^2 \sum_{n=0}^{\infty}  \left( \frac{t}{2} \right)^n   \]


Then the closed form would be


\[    \left( \frac{t}{2} \right)^2  \cdot \frac{1}{1 - \frac{t}{2}}            \]



\[     \frac{t^2}{2(2 - t)}            \]



Same formula.












\begin{example} Gemetric Series


Given 
\[    K(t) =   \sum_{n=0}^{\infty}  \left( \frac{t-3}{2} \right)^2\]

find the closed form formula and the interval of convergence.




\begin{explanation}


This is a Geometric series.  The interval of convergence is $(1, 5)$, since this is when the inside of the general term is $-1$ and $1$. Our interval is centered at $3$, which is where the terms equal $0$.


The closed form is

\[  \frac{1}{1 - \frac{t-3}{2}}  =     \frac{2}{2-(t-3)} =    \frac{2}{5-t}        \]



\end{explanation}


Our closed form formula has a singularity at $5$.  Therefore, our series equivalence cannot go beyond $5$, which it does not.




\begin{center}
\desmos{c3fj0aetfr}{400}{300}
\end{center}




\end{example}











\begin{center}
\textbf{\textcolor{green!50!black}{ooooo-=-=-=-ooOoo-=-=-=-ooooo}} \\

more examples can be found by following this link\\ \link[More Examples of Geometric Series]{https://ximera.osu.edu/csccmathematics/precalculus1/precalculus1/geometricSeries/examples/exampleList}

\end{center}



\end{document}
