\documentclass{ximera}

\input{../../preamble.tex}

\title{Disassemble}

\begin{document}

\begin{abstract}
taking apart
\end{abstract}
\maketitle





\begin{example}


Let $H(d)$ and $M(p)$ be two functions and $H \circ M$ be their composition.


Suppose $M(p) = 3 p - 5$ \\

Suppose $(H \circ M)(k) = 5 k + 1$


Find $H(d)$.



\begin{explanation}




$(H \circ M)(k) = H(M(k)) = H(3 k - 5)$  \\



$H$ is going to do something to $3 k - 5$ and produce $5 k + 1$. \\




These are both linear functions, therefore $H(d)$ should be a linear function.


First $H$ should multiply $3 k - 5$ by $\answer{\frac{5}{3}}$ to produce a $5k$.


\[    \frac{5}{3} (3 k - 5) = 5k - \frac{25}{3}   \]



Now, we need $-\frac{25}{3}$ to become $1$.  $H$ should add $\answer{\frac{28}{3}}$.

\[  H(d) =    \frac{5}{3} d +     \frac{28}{3} \]



$\blacktriangleright$ Check: 


\[    (H \circ M)(k) = H(M(k)) = H(3 k - 5) =    \frac{5}{3} (3 k - 5) +     \frac{28}{3}  = 5k - \frac{25}{3}  + \frac{28}{3}  = 5k + \frac{3}{3}  = 5k + 1\]





\end{explanation}

\end{example}













\begin{example}


Let $H(d)$ and $M(p)$ be two functions and $H \circ M$ be their composition.


Suppose $H(d) = 3 d - 5$ \\

Suppose $(H \circ M)(k) = 5 k + 1$


Find $M(p)$.



\begin{explanation}




$(H \circ M)(k) = H(M(k)) = 3 M(k) - 5 $  \\




These are both linear functions, therefore $M(k)$ should be a linear function.


$M$ is going to be multiplied by $3$, therefore $M$ should start with $M(p) = \answer{\frac{5}{3}}p$. That way, when it is multiplied by $3$, we will get $5p$.




Now, we need $3$ times something to be $1$.  $M$ should add $\answer{\frac{1}{3}}$.

\[  M(p) =    \frac{5}{3} p +     \frac{1}{3} \]



$\blacktriangleright$ Check: 


\[    (H \circ M)(k) = H(M(k)) = 3 \left( \frac{5}{3} k + \frac{1}{3} \right) - 5 =    5 k + 1    \]




\end{explanation} 

\end{example}










\begin{example}


Let $f(x)$ and $g(w)$ be two functions and $f \circ g$ be their composition.


Suppose $g(w) = 3w + 1$ \\

Suppose $(f \circ g)(t) = \frac{2t}{t-1}$


Find $f(x)$.



\begin{explanation}




$(f \circ g)(t) =  f(g(t)) =  \frac{2t}{t-1}$ \\



The composition has two occurrences of the variable.  $g$ has one occurrence and when it is put into $f$ the resulting formula has two occurrences.  It seems reasonable to guess that $f$ has two occurences of its variable - one in a numerator and one in a denominator.  $3t + 1$ will replace each in the composition.

So, let's start constructing. \\


$\blacktriangleright$  \textbf{\textcolor{blue!55!black}{Guess \#1)}}   \\

Let's start with two occurences of $x$, one in the numerator and one in the denominator.

\[      f(x) = \frac{x}{x}       \]


this makes the composition look like

\[   f(g(t)) =      \frac{3t + 1}{3t + 1}       \]



We need the coefficients of $t$ to be $2$ in the numerator and $1$ in the denominator.

$\blacktriangleright$  \textbf{\textcolor{blue!55!black}{Guess \#2)}}   \\

\[   f(g(t)) =      \frac{\answer{\frac{2}{3}}(3t + 1)}{\frac{1}{3}(3t + 1)}       \]

That gives


\[   f(g(t)) =      \frac{2t + \frac{2}{3}}{t + \frac{1}{3}}       \]



Now, we need constant terms of $0$ in the numerator and $-1$ in the denominator.  Subtract $\answer{\frac{2}{3}}$ from the numerator. Subtract $\answer{\frac{4}{3}}$ from the denominator. \\

$\blacktriangleright$  \textbf{\textcolor{blue!55!black}{Guess \#3)}}   \\


\[   f(g(t)) =      \frac{\frac{2}{3}(3t + 1) - \frac{2}{3}}{\frac{1}{3}(3t + 1) - \frac{4}{3}}       \]

That tells us what $f$ needs to do.




\[   f(x) =      \frac{\frac{2}{3}x - \frac{2}{3}}{\frac{1}{3}x - \frac{4}{3}}       \]



\end{explanation}

\end{example}























\begin{example}


Let $H(x)$ and $B(w)$ be two functions and $B \circ H$ be their composition.


Suppose $B(w) = 3w + 1$ \\

Suppose $(B \circ H)(t) = \frac{2t}{t-1}$


Find $H(x)$.



\begin{explanation}




$(B \circ H)(t) =  B(H(t)) = 3 H(t) + 1$ \\


We want this to equal $\frac{2t}{t-1}$.




\[
3 H(t) + 1 = \frac{2t}{t-1}
\]


We can solve for $H(t)$.



\[
3 H(t) + 1 = \frac{2t}{t-1}
\]

\[
3 H(t) = \frac{2t}{t-1} - 1 = \frac{\answer{t+1}}{t-1}
\]

\[
H(t)  = \answer{\frac{t+1}{3(t-1)}}
\]



Check:

\[
(B \circ H)(t) =  B(H(t)) = 3 H(t) + 1 = 3 \left( \frac{t+1}{3(t-1)} \right) + 1 = \frac{3(t+1) + 3(t-1)}{3(t-1)} 
\]


\[
 = \frac{(t+1) + (t-1)}{(t-1)}  = \frac{2t}{(t-1)}
\]



\end{explanation}

\end{example}





















\begin{center}
\textbf{\textcolor{green!50!black}{ooooo-=-=-=-ooOoo-=-=-=-ooooo}} \\

more examples can be found by following this link\\ \link[More Examples of Composition]{https://ximera.osu.edu/csccmathematics/precalculus1/precalculus1/composition/examples/exampleList}

\end{center}


\end{document}
